thys/Coinductive_Languages/CFG_Examples.thy
@@ -17,6 +17,7 @@ abbreviation "S \<equiv> Inr ()"
 
 interpretation palindromes!: cfg "()" "\<lambda>_. [[], [\<aa>], [\<bb>], [\<aa>, S, \<aa>], [\<bb>, S, \<bb>]]"
   by unfold_locales auto
+
 lemma "in_language palindromes.lang []" by normalization
 lemma "in_language palindromes.lang [True]" by normalization
 lemma "in_language palindromes.lang [False]" by normalization
@@ -24,10 +25,8 @@ lemma "in_language palindromes.lang [True, True]" by normalization
 lemma "in_language palindromes.lang [True, False, True]" by normalization
 lemma "\<not> in_language palindromes.lang [True, False]" by normalization
 lemma "\<not> in_language palindromes.lang [True, False, True, False]" by normalization
-(* slow
 lemma "in_language palindromes.lang [True, False, True, True, False, True]" by normalization
 lemma "\<not> in_language palindromes.lang [True, False, True, False, False, True]" by normalization
-*)
 
 interpretation Dyck!: cfg "()" "\<lambda>_. [[], [\<aa>, S, \<bb>, S]]"
   by unfold_locales auto
@@ -37,10 +36,19 @@ lemma "\<not> in_language Dyck.lang [False]" by normalization
 lemma "in_language Dyck.lang [True, False, True, False]" by normalization
 lemma "in_language Dyck.lang [True, True, False, False]" by normalization
 lemma "in_language Dyck.lang [True, False, True, False]" by normalization
-(* slow
 lemma "in_language Dyck.lang [True, False, True, False, True, True, False, False]" by normalization
-*)
 lemma "\<not> in_language Dyck.lang [True, False, True, True, False]" by normalization
 lemma "\<not> in_language Dyck.lang [True, True, False, False, False, True]" by normalization
+
+interpretation abSSa!: cfg "()" "\<lambda>_. [[], [\<aa>, \<bb>, S, S, \<aa>]]"
+  by unfold_locales auto
+lemma "in_language abSSa.lang []" by normalization
+lemma "\<not> in_language abSSa.lang [True]" by normalization
+lemma "\<not> in_language abSSa.lang [False]" by normalization
+lemma "in_language abSSa.lang [True, False, True]" by normalization
+lemma "in_language abSSa.lang [True, False, True, False, True, True, False, True, True]" by normalization
+lemma "in_language abSSa.lang [True, False, True, False, True, True]" by normalization
+lemma "\<not> in_language abSSa.lang [True, False, True, True, False]" by normalization
+lemma "\<not> in_language abSSa.lang [True, True, False, False, False, True]" by normalization
 
 end
